veric/align_mem.v
@@ -1,0 +1,238 @@
+Require Import VST.msl.msl_standard.
+Require Import VST.veric.base.
+Require Import VST.veric.rmaps.
+Require Import VST.veric.compcert_rmaps.
+Require Import VST.veric.Clight_lemmas.
+Require Export VST.veric.lift.
+
+(* This file contains two align criteria: a strong one and a weak one.
+   The strong one derives alignment of types from align_memdata.
+   The weak one only requires every single field to be well aligned. *)
+
+(* Aux: relative_complete_type *)
+
+Fixpoint relative_complete_type {A: Type} (env: PTree.t A) (t: type): bool :=
+  match t with
+  | Tvoid => false
+  | Tint _ _ _ => true
+  | Tlong _ _ => true
+  | Tfloat _ _ => true
+  | Tpointer _ _ => true
+  | Tarray t' _ _ => relative_complete_type env t'
+  | Tfunction _ _ _ => false
+  | Tstruct id _ => match env ! id with
+                    | Some _ => true
+                    | None => false
+                    end
+  | Tunion id _ => match env ! id with
+                   | Some _ => true
+                   | None => false
+                   end
+  end.
+
+Print Build_composite.
+Print make_composite_env.
+Print build_composite_env.
+Print add_composite_definitions.
+(* Aux: composite_env's PTree members reordering *)
+
+Definition PTree_get_list {A: Type} (i: positive) (T: PTree.t (list A)): list A :=
+  match PTree.get i T with
+  | Some l => l
+  | None => nil
+  end.
+
+Definition PTree_set_cons {A: Type} (i: positive) (a: A) (T: PTree.t (list A)) :=
+  PTree.set i (a :: PTree_get_list i T) T.
+
+Definition rebuild_composite_tree (env: composite_env): PTree.t (list (ident * composite)) :=
+  fold_right (fun ic => PTree_set_cons (Pos.of_succ_nat (co_rank (snd ic))) ic) (PTree.empty _) (PTree.elements env).
+
+Definition max_rank_composite (env: composite_env): nat :=
+  fold_right (fun ic => max (co_rank (snd ic))) O (PTree.elements env).
+
+Lemma max_rank_composite_is_upper_bound: forall env i co,
+  PTree.get i env = Some co ->
+  (co_rank co <= max_rank_composite env)%nat.
+Proof.
+  intros.
+  apply PTree.elements_correct in H.
+  unfold max_rank_composite.
+  induction (PTree.elements env).
+  + inv H.
+  + destruct H.
+    - subst.
+      simpl.
+      apply Max.le_max_l.
+    - apply IHl in H.
+      etransitivity; [exact H |].
+      simpl.
+      apply Max.le_max_r.
+Qed.
+
+(* Strong align requirement *)
+Fixpoint plain_alignof (env_al: PTree.t Z) t: Z :=
+  match t with
+  | Tvoid
+  | Tfunction _ _ _ => 1
+  | Tint I8 _ _ => 1
+  | Tint I16 _ _ => 2
+  | Tint I32 _ _ => 4
+  | Tint IBool _ _ => 1
+  | Tlong _ _ => 8
+  | Tfloat F32 _ => 4
+  | Tfloat F64 _ => 4
+  | Tpointer _ _ => 4
+  | Tarray t' _ _ => plain_alignof env_al t'
+  | Tstruct id _ =>
+      match env_al ! id with
+      | Some al => al
+      | None => 1
+      end
+  | Tunion id _ =>
+      match env_al ! id with
+      | Some al => al
+      | None => 1
+      end
+  end.
+
+Print composite_env.
+Print composite.
+Print compcert.cfrontend.Ctypes.composite_env_consistent.
+Print composite_consistent.
+Print alignof_composite.
+
+Fixpoint plain_alignof_composite (env_al: PTree.t Z) (m: members): Z :=
+  match m with
+  | nil => 1
+  | (_, t) :: m' => Z.max (plain_alignof env_al t) (plain_alignof_composite env_al m')
+  end.
+
+Definition composites_plain_alignof_S (l: list (positive * composite)) (env_al: PTree.t Z) :=
+  fold_right (fun ic => PTree.set (fst ic) (plain_alignof_composite env_al (co_members (snd ic)))) env_al l.
+
+Definition composites_plain_alignof_rec (env: composite_env) T: nat -> PTree.t Z :=
+  fix composites_plain_alignof_rec (n: nat): PTree.t Z :=
+    match n with
+    | O => PTree.empty _
+    | S n' => composites_plain_alignof_S (PTree_get_list (Pos.of_succ_nat n') T) (composites_plain_alignof_rec n')
+    end.
+
+Definition composites_plain_alignof (env: composite_env): PTree.t Z :=
+  let T := rebuild_composite_tree env in
+  composites_plain_alignof_rec env T (S (max_rank_composite env)).
+
+Definition consistent_plain_alignof env env_al: Prop :=
+  forall i al co,
+    PTree.get i env_al = Some al ->
+    PTree.get i env = Some co ->
+    al = plain_alignof_composite env_al (co_members co).
+
+Lemma composites_plain_alignof_S_fact: forall l env env_al,
+  consistent_plain_alignof env env_al ->
+  (forall i co r list_r, In (i, co) l -> PTree.get env_al r = Some list_r ->
+     In (i, co) list_r 
+    
+Lemma co_consistent_plain_alignof: forall env env_al,
+  env_al = composites_plain_alignof env ->
+  composite_env_consistent env ->
+  consistent_plain_alignof env env_al.
+Proof.
+  intros.  
+  cbv zeta beta delta [composites_plain_alignof] in H.
+  set (RCT := rebuild_composite_tree env) in H.
+  pose proof max_rank_composite_is_upper_bound env _ _ H2.
+  apply le_lt_n_Sm in H3.
+  subst env_al.
+  revert i al co H1 H2 H3; induction (S (max_rank_composite env)); intros.
+  + clear - H3; exfalso. omega.
+  + set (CPA := composites_plain_alignof_rec env RCT n) in IHn.
+    change (composites_plain_alignof_rec env RCT (S n)) with (composites_plain_alignof_S (PTree_get_list (Pos.of_succ_nat n) RCT) CPA) in H1 |- *.
+
+
+
+
+
+
+
+
+
+
+
+
+
+
+
+
+    
+    Locate op
+
+Lemma plain_alignof_spec: forall env t,
+  alignof env t = align_attr (attr_of_type t) (plain_alignof env t).
+Proof.
+  intros.
+  destruct t; auto.
+Qed.
+
+Lemma plain_alignof_two_p: forall env t, exists n,
+  plain_alignof env t = two_power_nat n.
+Proof.
+  intros.
+  destruct t as [| []  ? ? | | [] ? | | | | |];
+  try solve [exists 0%nat; reflexivity | exists 1%nat; reflexivity | exists 2%nat; reflexivity].
+  + simpl.
+    apply alignof_two_p.
+  + simpl.
+    destruct (env ! i); [apply co_alignof_two_p | exists 0%nat; auto].
+  + simpl.
+    destruct (env ! i); [apply co_alignof_two_p | exists 0%nat; auto].
+Qed.
+
+Definition local_legal_alignas_type env (t: type): bool :=
+  Z.leb (plain_alignof env t) (alignof env t) &&
+  match t with
+  | Tarray t' n a => Z.eqb ((sizeof env t') mod (alignof env t')) 0 && Z.leb 0 n
+  | Tlong _ _ => Z.leb 8 (alignof env t)
+  | _ => true
+  end.
+
+Lemma local_legal_alignas_type_spec: forall env t,
+  local_legal_alignas_type env t = true ->
+  (plain_alignof env t | alignof env t).
+Proof.
+  intros.
+  apply andb_true_iff in H.
+  destruct H as [? _].
+  apply Zle_is_le_bool in H.
+  apply power_nat_divide'; [apply alignof_two_p | apply plain_alignof_two_p | omega].
+Qed.
+
+Lemma align_chunk_alignof: forall env t ch, local_legal_alignas_type env t = true -> access_mode t = By_value ch -> (Memdata.align_chunk ch | alignof env t).
+Proof.
+  intros.
+  destruct t; inversion H0.
+  - eapply Z.divide_trans; [| apply local_legal_alignas_type_spec; auto].
+    destruct i, s; inversion H2; simpl; unfold align_attr;
+    destruct (attr_alignas a); reflexivity.
+  - unfold local_legal_alignas_type in H.
+    rewrite andb_true_iff in H; destruct H as [_ ?].
+    apply Zge_is_le_bool in H.
+    apply power_nat_divide' in H.
+    * auto.
+    * apply alignof_two_p.
+    * exists 3%nat; auto.
+  - eapply Z.divide_trans; [| apply local_legal_alignas_type_spec; auto].
+    destruct f; inversion H2; simpl; unfold align_attr;
+    destruct (attr_alignas a); reflexivity.
+  - eapply Z.divide_trans; [| apply local_legal_alignas_type_spec; auto].
+    inversion H2; simpl; unfold align_attr;
+    destruct (attr_alignas a); reflexivity.
+Qed.
+
+Definition composite_legal_alignas (env : composite_env) (co : composite) : Prop :=
+  (co_alignof co >= alignof_composite env (co_members co)).
+
+Definition composite_env_legal_alignas env :=
+  forall (id : positive) (co : composite),
+    env ! id = Some co -> composite_legal_alignas env co.
+
