veric/composite_compute.v
@@ -1,0 +1,66 @@
+Require Import Coq.Sorting.Permutation.
+Require Import VST.veric.base.
+Require Import VST.veric.Clight_lemmas.
+
+Fixpoint relative_defined_type {A: Type} (l: list (ident * A)) (t: type): Prop :=
+  match t with
+  | Tarray t' _ _ => relative_defined_type l t'
+  | Tstruct id _ => In id (map fst l)
+  | Tunion id _ => In id (map fst l)
+  | _ => True
+  end.
+
+Module type_func.
+Section type_func.
+
+Context {A: Type}
+        (f_default: type -> A)
+        (f_array: A -> Z -> attr -> A)
+        (f_struct: A -> attr -> A)
+        (f_union: A -> attr -> A)
+        (f_member: struct_or_union -> list (ident * A) -> A).
+
+Fixpoint F (env: PTree.t A) (t: type): A :=
+  match t with
+  | Tarray t n a => f_array (F env t) n a
+  | Tstruct id a =>
+      match env ! id with
+      | Some v => f_struct v a
+      | None => f_default t
+      end
+  | Tunion id a =>
+      match env ! id with
+      | Some v => f_union v a
+      | None => f_default t
+      end
+  | _ => f_default t
+  end.
+
+Fixpoint Env (l: list (positive * composite)): PTree.t A :=
+  fold_right
+    (fun (ic: positive * composite) env =>
+       let (i, co) := ic in
+       PTree.set i
+                 (f_member (co_su co)
+                           (map
+                              (fun it0: positive * type =>
+                                 let (i0, t0) := it0 in (i0, F env t0))
+                              (co_members co)))
+                 env)
+    (PTree.empty A)
+    l.
+
+Lemma Consistent: forall env l,
+  Permutation l (PTree.elements env) ->
+  (forall l1 i co l2,
+      l = l1 ++ (i, co) :: l2 ->
+      Forall (relative_defined_type l1) (map snd (co_members co))) ->
+  forall i co a,
+    PTree.get i env = Some co ->
+    PTree.get i (Env (PTree.elements env)) = Some a ->
+    a = f_member (co_su co) (map
+                              (fun it0: positive * type =>
+                                 let (i0, t0) := it0 in
+                                 (i0, F (Env l) t0))
+                              (co_members co)).
+                 .
